programs/lean/Project.lean
@@ -1,3 +1,4 @@
 import Project.NumInteger.Spec
 import Project.RustU64.Spec
+import Project.RustU64Tests.Spec
 import Project.TotalVariation.Spec
